Finished select_with_max for List.Greedy

FormalMatroidOptimization/Greedy/Basic.lean
@@ -7,34 +7,37 @@ open List
 
 namespace Greedy
 
-def selectRel_internal {α : Type*} [DecidableEq α] (P : Finset α → Bool) (r : α → α → Prop)
-    [DecidableRel r] [IsTotal α r] [IsTrans α r] (s indep : List α) : List α :=
-  let sP := s.filter (fun x ↦ P (insert x indep.toFinset))
+variable {α : Type*} [DecidableEq α]
+
+def selectRel_internal (P : Finset α → Prop) [DecidablePred P] (r : α → α → Prop) [DecidableRel r]
+    [IsTotal α r] [IsTrans α r] (xs ys : List α) : List α :=
+  let sP := xs.filter (fun x ↦ P (insert x ys.toFinset))
   if hsP : sP ≠ [] then
     let y := sP.maxRel r hsP
-    selectRel_internal P r (s.erase y) (y :: indep)
+    selectRel_internal P r (xs.erase y) (y :: ys)
   else
-    indep
+    ys
   termination_by
-    s.length
+    xs.length
   decreasing_by
     apply Order.lt_of_succ_lt_succ
     rw [Order.succ_eq_add_one, List.length_erase_add_one ?_]
     · simp
-    · have : (filter (fun x ↦ P (insert (↑x) indep.toFinset)) s.attach).unattach ⊆ s := by simp
+    · have : (filter (fun x ↦ P (insert (↑x) ys.toFinset)) xs.attach).unattach ⊆ xs := by
+        intro z hz; simp at hz; exact hz.left
       exact this (maxRel_mem r hsP)
 
-def selectRel {α : Type*} [DecidableEq α] (P : Finset α → Bool) (r : α → α → Prop) [DecidableRel r]
-    [IsTotal α r] [IsTrans α r] (lst : List α) : List α :=
-  selectRel_internal P r lst ∅
+def selectRel (P : Finset α → Prop) [DecidablePred P] (r : α → α → Prop) [DecidableRel r]
+    [IsTotal α r] [IsTrans α r] (xs : List α) : List α :=
+  selectRel_internal P r xs []
 
-@[simp] theorem selectRel_nil {α : Type*} [DecidableEq α] (P : Finset α → Bool) (r : α → α → Prop)
-    [DecidableRel r] [IsTotal α r] [IsTrans α r] : selectRel P r [] = [] := by
+@[simp] theorem selectRel_nil {P : Finset α → Prop} [DecidablePred P]
+    {r : α → α → Prop} [DecidableRel r] [IsTotal α r] [IsTrans α r] : selectRel P r [] = [] := by
   simp [selectRel, selectRel_internal]
 
-theorem selectRel_internal_subset {α : Type*} [DecidableEq α] (P : Finset α → Prop)
-    [DecidablePred P] (r : α → α → Prop) [DecidableRel r] [IsTotal α r] [IsTrans α r] {xs : List α}
-    {ys : List α} :
+
+theorem selectRel_internal_subset {P : Finset α → Prop} [DecidablePred P]
+    {r : α → α → Prop} [DecidableRel r] [IsTotal α r] [IsTrans α r] {xs ys : List α} :
     ys ⊆ selectRel_internal P r xs ys := by
   match xs with
   | [] =>
@@ -44,7 +47,7 @@ theorem selectRel_internal_subset {α : Type*} [DecidableEq α] (P : Finset α �
     set sP := filter (fun x ↦ decide (P (insert x ys.toFinset))) (x :: xs) with hsP₁
     by_cases hsP₂ : sP ≠ []
     · rw [dif_pos hsP₂]
-      exact subset_of_cons_subset (selectRel_internal_subset P r
+      exact subset_of_cons_subset (selectRel_internal_subset
         (xs := ((x :: xs).erase (List.maxRel r sP hsP₂))) (ys := ((List.maxRel r sP hsP₂) :: ys)))
     · rw [dif_neg hsP₂]
       simp
@@ -53,10 +56,11 @@ theorem selectRel_internal_subset {α : Type*} [DecidableEq α] (P : Finset α �
   decreasing_by
     grind [List.maxRel_mem]
 
-theorem selectRel_internal_indep {α : Type*} [DecidableEq α] (P : Finset α → Prop) [DecidablePred P]
-    (r : α → α → Prop) [DecidableRel r] [IsTotal α r] [IsTrans α r] {xs : List α} {ys : List α}
-    (hys : P ys.toFinset) : P (selectRel_internal P r xs ys).toFinset := by
-    match xs with
+theorem selectRel_internal_indep {P : Finset α → Prop} [DecidablePred P]
+    {r : α → α → Prop} [DecidableRel r] [IsTotal α r] [IsTrans α r]
+    {xs ys : List α} (hys : P ys.toFinset) :
+    P (selectRel_internal P r xs ys).toFinset := by
+  match xs with
   | [] =>
     grind [selectRel_internal]
   | x :: xs =>
@@ -64,7 +68,7 @@ theorem selectRel_internal_indep {α : Type*} [DecidableEq α] (P : Finset α �
     set sP := filter (fun x ↦ decide (P (insert x ys.toFinset))) (x :: xs) with hsP₁
     by_cases hsP₂ : sP ≠ []
     · rw [dif_pos hsP₂]
-      apply (selectRel_internal_indep P r
+      apply (selectRel_internal_indep
         (xs := ((x :: xs).erase (List.maxRel r sP hsP₂))) (ys := ((List.maxRel r sP hsP₂) :: ys)))
       have := (mem_filter.mp (maxRel_mem r hsP₂)).right
       rw [Bool.decide_iff] at this
@@ -75,10 +79,45 @@ theorem selectRel_internal_indep {α : Type*} [DecidableEq α] (P : Finset α �
   decreasing_by
     grind [List.maxRel_mem]
 
-theorem selectRel_internal_with_max {α : Type*} [DecidableEq α] (P : Finset α → Prop)
-    [DecidablePred P] (hP : IndepSystem.HereditaryProperty P) (r : α → α → Prop) [DecidableRel r]
-    [IsTotal α r] [IsTrans α r] {x : α} {xs : List α} {ys : List α}
-    (h : ∀ y ∈ xs, r y x ∧ ¬r x y) :
+theorem selectRel_internal_prop
+    {P : Finset α → Prop} [DecidablePred P] (hP : IndepSystem.HereditaryProperty P)
+    {r : α → α → Prop} [DecidableRel r] [IsTotal α r] [IsTrans α r]
+    {xs ys : List α} :
+    selectRel_internal P r xs ys = (selectRel_internal (fun s ↦ P (s ∪ ys.toFinset)) r xs []) ++ ys
+    := by
+  rw [selectRel_internal.eq_def, selectRel_internal.eq_def]
+  set sP := filter (fun x ↦ decide (P (insert x ys.toFinset))) xs with hsP₁
+  have : sP = filter (fun x ↦ decide (P (insert x [].toFinset ∪ ys.toFinset))) xs := by rfl
+  rw [← this]
+  by_cases hsP₂ : sP ≠ []
+  · rw [dif_pos hsP₂, dif_pos hsP₂]
+    have := selectRel_internal_prop (r := r) (xs := (xs.erase (List.maxRel r sP hsP₂)))
+      (ys := (List.maxRel r sP hsP₂) :: ys) hP
+    rw [this]
+    set P₁ := fun s ↦ P (s ∪ ys.toFinset) with hP₁
+    have hP₂ : IndepSystem.HereditaryProperty P₁ := by
+      intro X Y hX hXY
+      simp only [hP₁] at hX ⊢
+      have : (Y ∪ ys.toFinset) ⊆ (X ∪ ys.toFinset) := by grind
+      exact hP hX this
+    have := selectRel_internal_prop (r := r) (xs := (xs.erase (List.maxRel r sP hsP₂)))
+      (ys := [List.maxRel r sP hsP₂]) hP₂
+    rw [this, ← singleton_append, append_assoc]
+    congr
+    ext x
+    simp [hP₁]
+  · rw [dif_neg hsP₂, dif_neg hsP₂]
+    simp
+  termination_by
+    xs.length
+  decreasing_by
+    · grind [List.maxRel_mem]
+    · grind [List.maxRel_mem]
+
+theorem selectRel_internal_with_max
+    {P : Finset α → Prop} [DecidablePred P] (hP : IndepSystem.HereditaryProperty P)
+    {r : α → α → Prop} [DecidableRel r] [IsTotal α r] [IsTrans α r]
+    {x : α} {xs ys : List α} (h : ∀ y ∈ xs, r y x ∧ ¬r x y) :
     if P (insert x ys.toFinset) then
       selectRel_internal P r (x :: xs) ys = selectRel_internal P r xs (x :: ys)
     else
@@ -105,7 +144,8 @@ theorem selectRel_internal_with_max {α : Type*} [DecidableEq α] (P : Finset α
         rw [erase_cons_tail ?_]
         have := Finset.forall_mem_not_eq.mpr ((not_iff_not.mpr (List.mem_toFinset)).mpr hx)
         simp [hy₁, (this (List.maxRel r sP hsP₂) (by simp [maxRel_mem r hsP₂]))]
-      have  h' := selectRel_internal_with_max P hP r ?_ (x := x) (xs := xs.erase y) (ys := y :: ys)
+      have  h' := selectRel_internal_with_max hP ?_
+        (r := r) (x := x) (xs := xs.erase y) (ys := y :: ys)
       · by_cases hP₂ : P (insert x (y :: ys).toFinset)
         · have : (insert x ys.toFinset) ⊆ (insert x (y :: ys).toFinset) := by simp
           exact False.elim (hP₁ (hP hP₂ this))
@@ -117,20 +157,22 @@ theorem selectRel_internal_with_max {α : Type*} [DecidableEq α] (P : Finset α
   decreasing_by
     grind [List.maxRel_mem]
 
-theorem selectRel_with_max {α : Type*} [DecidableEq α] (P : Finset α → Prop)
-    [DecidablePred P] (hP : IndepSystem.HereditaryProperty P) (r : α → α → Prop) [DecidableRel r]
-    [IsTotal α r] [IsTrans α r] {x : α} {xs : List α} (h : ∀ y ∈ xs, r y x ∧ ¬r x y) :
+theorem selectRel_with_max
+    {P : Finset α → Prop} [DecidablePred P] (hP : IndepSystem.HereditaryProperty P)
+    {r : α → α → Prop} [DecidableRel r] [IsTotal α r] [IsTrans α r]
+    {x : α} {xs : List α} (h : ∀ y ∈ xs, r y x ∧ ¬r x y) :
     if P {x} then
-      selectRel P r (x :: xs) = selectRel_internal P r xs [x]
+      selectRel P r (x :: xs) = selectRel (fun s ↦ P (s ∪ {x})) r xs ++ [x]
     else
       selectRel P r (x :: xs) = selectRel P r xs
     := by
   unfold selectRel
-  have := selectRel_internal_with_max P hP r h (ys := [])
+  have := selectRel_internal_with_max hP h (ys := [])
   have h₁ : (insert x [].toFinset) = {x} := by rw [toFinset_nil, insert_empty_eq]
   rw [h₁] at this
   by_cases hP₁ : P {x}
-  · rwa [if_pos hP₁] at this ⊢
+  · rw [if_pos hP₁] at this ⊢
+    simp [this, selectRel_internal_prop hP]
   · rwa [if_neg hP₁] at this ⊢
 
 end Greedy
